Monad_Play Around/State_Monad_EX.thy
@@ -51,9 +51,31 @@ definition q0:: "S1 \<Rightarrow> bool" where "q0 s = (x_S1 s = y_S1 s \<and> x_
 definition q1:: "unit \<Rightarrow> S1 \<Rightarrow> bool" where "q1 _ s = (x_S1 s = y_S1 s)"
 
 lemma "spec TT let0 (GG q0)"
-  apply (simp add: let0_def GG_def)
-  apply (intro seq_rule[of _ _ "\<lambda>_ s. (x_S1 s = y_S1 s)"])
-   apply (simp add: spec_def TT_def q1_def assign_def return_def get_def put_def get_state_def put_state_def y_S1u_def)
-  by (simp add: spec_def GG_def q0_def assign_def get_def return_def put_def get_state_def put_state_def z_S1u_def)
+  apply (simp add: let0_def)
+  apply (intro seq_rule[of _ _ "q1"])
+   apply (simp add: spec_def q1_def assign_def return_def get_def put_def get_state_def put_state_def y_S1u_def)
+  by (simp add: spec_def GG_def q1_def q0_def assign_def get_def return_def put_def get_state_def put_state_def z_S1u_def)
 
+definition ifc0:: "(S1, unit) state" where "ifc0 = do { c \<leftarrow> get x_S1; if c < 0 then assign y_S1u x_S1 else assign z_S1u x_S1 }"
+
+definition q2:: "S1 \<Rightarrow> bool" where "q2 s = (x_S1 s = z_S1 s)"
+
+lemma "spec (\<lambda>s. x_S1 s > 0) ifc0 (GG q2)"
+  apply (simp add: ifc0_def)
+  apply (intro get_rule)
+  apply (intro allI)
+  apply (intro cond_rule)
+   apply (simp add: spec_def assign_def get_def get_state_def return_def put_def put_state_def GG_def q2_def)
+  by (simp add: spec_def assign_def get_def get_state_def return_def put_def put_state_def GG_def q2_def z_S1u_def)
+
+definition dec0:: "(S1, unit) state" where "dec0 = do { assign z_S1u x_S1; assign x_S1u (\<lambda>x. x_S1 x - 1) }"
+
+definition p3:: "int \<Rightarrow> S1 \<Rightarrow> bool" where "p3 N s = (x_S1 s = N)"
+definition q3:: "int \<Rightarrow> S1 \<Rightarrow> bool" where "q3 N s = (x_S1 s < N \<and> z_S1 s = N)"
+
+lemma "spec (p3 N) dec0 (GG (q3 N))"
+  apply (simp add: dec0_def)
+  apply(intro seq_rule[of _ _ "\<lambda>_ s. x_S1 s = N \<and> z_S1 s = N"])
+  apply (simp add: spec_def assign_def put_def get_def get_state_def put_state_def return_def z_S1u_def p3_def)
+  by (simp add: spec_def assign_def put_def get_def get_state_def put_state_def return_def x_S1u_def GG_def q3_def)
 end
